---
title: 1. U-Substitution
editor: 
  markdown: 
    wrap: 72
---

-   Let $u = x^3 + 1$

Then $du = 3x^2 dx$

-   Solve for $dx$:

$dx = \frac{du}{3x^2}$

Check:

-   Write the integral in terms of $u$:

$$
\begin{align*}
  \int 3^2 (x^3+1) dx = \int 3^2 (x^3 + 1) \frac{du}{3x^2} \\
  \int {} \\
\end{align*}
$$

E1

Let $u = x^2 + 1$, then $du = 2xdx$

$\qquad dx = \frac{dx = \frac{du}{2x}$

$$
\begin{align*}
   \int 2x \sqrt{x^2+1} dx \\
   \int 2x \sqrt{x^2+1} \frac{du}{2x} \\
\end{align*}
$$

E?

$$
\begin{align*}
  \int x^2 (x^3 + 1)^4 dx \\
  u = x^3 + 1 \implies du = 3x^2 dx \\
  \implies dx = \frac{du}{3x^2} \\ 
  \implies \int x^2 (x^3 + 1)^4 dx = \int x^2 (x^3 + 1)^4 \frac{du}{3x^2} \\
  \\
\end{align*}
$$

E3

$$
\begin{align*}
  \int 10x^2 \sqrt{x^3+1} dx \\
  u = x^3 + 1 \implies du = 3x^2 dx \\
  \boxed{dx = \frac{du}{3x^2}} \\
  \implies \int 10x^2 \sqrt{x^3+1} dx = \int 10\cancel{x^2} \sqrt{x^3+1} \frac{du}{3\cancel{x^2}} \\
\end{align*}
$$

Look at the following integrals:

$$\int3x^2\left(x^3+1\right)^4dx\quad\int2x\sqrt{x^2+1}\:dx\quad\int\frac{4x^3}{\left(x^4+1\right)^3}dx$$

Notice anything?Each expression is a function and it's derivative.

![](u1-u-substitution-img/fsUngrEkOhHpglocXIb4LDYRprbCNi6Lg)

$$\frac{d}{dx}f(g(x))=f'\bigl(g(x)\bigr)g'(x)$$

If we see this pattern, we can use U-substitution to find the integral.

To integrate $\int3x^{2}\left(x^{3}+1\right)^{4}dx$ we need to rewrite
it to see the parts of the derivative

Check:

### PROCEDURE FOR U-SUBSTITUTION

1.Carefully define a new function, $lu$ ,(it will be the inside
function).

1. Find its differential, $du$ . 3.Rewrite the original function in
    terms of $\iota\iota$ and $du$

------------------------------------------------------------------------

E1 Find the indefinite integral $\int 2x\sqrt {x^{2}+ 1}$ $dx$

E in teteae $\int\frac{4x^3dx}{\left(x^4+2\right)^3}$

Check:

------------------------------------------------------------------------

Often we will need to use a constant multiple to make the substitution
work. GET GOoD ATTHIS

$$\int x^2(x^3+1)^4dx$$

3 Find the indefinite integral, confirm your result by taking the
derivative

a) $\int 10x^{2}\sqrt {x^{3}+ 1}$ $dx$

$$\text{b)}\int\frac{x^3}{2\left(x^4+2\right)^3}dx\:.$$

------------------------------------------------------------------------

## Exponential Functions

For the function $e^x$

$$\frac{d}{dx}(e^x)=$$

So, going backwards, we know

![](u1-u-substitution-img/ff3tvNSMIkgG87GyXOmbufWON2AGGpUYi)

From the chain rule for $e^{f(x)}$

$$\frac{de^{f(x)}}{dx}=$$

So:

$$\int e^{f(x)}f'(x)dx=$$

![](u1-u-substitution-img/fSoipa5WephCL4c8wS8TtpicH3xcSdPH2)

We can use U Substitution to make the process easier.

### NATURAL EXPONENTIAL RULE

Weintegratefunctions with a natural base of $e$ using this rule.

$$\int e^{f(x)}f'(x)dx=e^{f(x)}+C$$

------------------------------------------------------------------------

E1Find the integral of the following functions and check your answers by
differentiation. $$f(t)=\frac{1}{3}e^{t}$$

$${\bar{f}}(x)={\frac{e^{x}}{5}}$$

(a) $f(x)=4e^x$ (b)

E2 Find the integral of the following functions and check your answers
by differentiation

a) $f(x)=4e^{3x}$

$$
\begin{align*}
 \int  \\
\end{align*}
$$

a) $)f(x) = x^{2}\frac{ e^{2x^3} }{5}$

$$
\begin{align*}
  u =  \\
\end{align*}
$$

E3 Find the particular solution of the function $f(x)$ When its curve
pass through the point $\left(1,\frac{e^{2}}{30}\right)$
$$f(x)=\int\frac{1}{3}xe^{5x^{2}-3}dx$$

$$
\begin{align*}
  u = 5x^2-3 \implies du = 10x dx \\
  \implies \boxed{ dx = \frac{du}{10x} } \\
  implies f(x)=\int\frac{1}{3}xe^{5x^{2}-3}dx = \int\frac{1}{3} \cancel{x} e^{5x^{2}-3} \frac{du}{10\cancel{x}} \\
  f(x) = \frac{1}{30} \int e^{ u } du \\
  f(x) = \frac{1}{30} e ~inc \\
\end{align*}
$$

------------------------------------------------------------------------

For the function $a^{x}$

So, we know:

$$\int a^x\ln(a)dx=$$

$$\frac{da^x}{dx}=$$

![](u1-u-substitution-img/fRPXTxnaokIS7EzdSQ7ewgpadSgQWB6eK)

From the chain rule for $a^{f(x)}$

So:

![](u1-u-substitution-img/fyT5WCUpgYcBqNdFDzoS5HRyY9KEGSfdy)

$$\begin{matrix}\int a^{f(x)}\ln(a)f'(x)\:dx=\end{matrix}$$

![](u1-u-substitution-img/fQoUNAHOZQgkpzGC29gwwKGux7MyqDuBH)

### GENERAL EXPONENTIAL RULE

We integrate functions whose base is any constant, $a$ using thisrule.

$$\int a^{f(x)}\ln\lvert a\rvert f'(x)dx=a^{f(x)}+C$$

------------------------------------------------------------------------

E3Find the integral of the following functions.

$$\text{b)}f\left(x\right)=12^x$$

$$\int5^{x}\ln(5)dx$$

a) $f(x)=7^{x^2}\ln(7)2x$

$$\int x^{2}\cdot3^{x^{3}}dx$$

$$\text{f)}\int5^{x^2+x}(4x+2)dx$$

------------------------------------------------------------------------

### 1.3 Natural Logarithms.

We know te deriatie o the aturl lgaritmi unctinn
$\frac{d}{dx}\ln x=\frac{1}{x}$

For the antiderivative however, we need to consider the functions

$$f(x)=\ln x$$

![](u1-u-substitution-img/frhtEnaaAZSFFQdclcTVp7K8xk9QhakUk)

![](u1-u-substitution-img/fnYvIWACUEbT2IBtcVnlZzVsMp37uZ068)

Now,for the function $\ln(f(x))$

So, we know:

$$\frac{d}{dx}\ln(f(x))=$$

$$\int\frac{1}{f(x)}f'(x)dx=$$

SO

$$\int\frac{1}{x}dx=$$

![](u1-u-substitution-img/fGvI2z46w5kYirbXUFc6HhWtZtGKybUOR)

If we see this pattern,

U-substitution is still used for logarithms. For a function that is a
quotient: $$f\begin{pmatrix}x\end{pmatrix}=\frac{6x+6}{3x^2+6x}$$

we have a Ln function as the antiderivative.

### "Ln" RULE

If a quotient can be manipulated with u-substitution to be a function in
the denominator with its derivative in the numerator then:
$$\int\frac{1}{f(x)}f'(x)dx=\ln\left|f(x)\right|+C$$

Remember:thatyou need to add the absolute value symbols to your integral

------------------------------------------------------------------------

E1 Find the integral of the following functions

$$\mathrm{b)}\int\frac{1}{11}t^{-1}dt$$

a) $\int\frac4xdx$

$$\text{c)}\int\frac{1}{3(x-5)}dx$$

Remember: you may need a constant multiple to make the rule work.

E2 Find the integral of the following using U substitution

$$)\:\int\frac{2t+1}{3t^{2}+3t}dt$$

$$\text{b)}\int\frac{x^4}{2x^5+2}dx$$

E3 Find the paricular olution of $\mathbf{v}=\int\frac{1}{2x+1}dx$ when
$x=0$ and $y=2$

------------------------------------------------------------------------

Things to look for:.

$$\frac{3x^3+3x}{x^4+3x^2+2x}$$

The quotient could use $$\frac{2e^{2x}+1}{e^{2x}+x}$$ other rules as
well:.

Be careful if you see a log in the denominator! We solve these a little
differently. Usually, $u=\ln x$ 1

$$\int\frac{1}{x(\ln x)^2}dx$$

------------------------------------------------------------------------

E3Simplify the following integrals if necessary and solve

$$)\:\int\frac{x(x-1)}{2x^{3}-3x^{2}}dx$$

$$\text{b)}\int\frac{2x-2}{\left(x-1\right)^{2}}dx$$

$$\text{c)}\int\frac{e^{2x}}{e^x(e^x+1)}dx$$

$$)\:\int\frac{1}{x\ln(x^{2})}dx$$

------------------------------------------------------------------------

## 1.4 Trigonometric Functions

We know the [derivatives of the basic trigonometric
functions](../../sem2/calc1/u3-transcendental.qmd##%20The%20Derivative%20of%20Trigonometric%20Functions)

Working backwards from these will lead us to integrals of the most basic
trigonometric functions.

### BASIC TRIGONOMETRIC INTEGRALS

$$
\begin{array}{c|c@{}c}
    f(x) & & F(x) \\
    \hline
    \cos x && \sin x + c \\
    \sin x & - & \cos x + c \\
    \sec x \cdot \sec x && \tan x + c \\
    \tan x \cdot \sec x && \sec^2 x + c \\
    \csc x \cdot \csc x \\
    \cot x \cdot \csc x \\
    e^x  \\
    \ln x & &\dfrac{1}{x} \\
\end{array}
$$

------------------------------------------------------------------------

E1 Find the indefinite integralof each of the following.

a) $\int 4 \sin x dx$

$= -4 \cos x + c$

a) $\int\sec(2x)\tan(2x)dx$

$$\begin{align*}
  \text{Let } u = 2x \implies du = 2 dx \\
  \therefore \frac{1}{2} \int \sec u \tan u~du \\
  = \frac{1}{2} \sec u + c \\
  = \boxed{\frac{1}{2} \sec 2x +c} \\
\end{align*}$$

<details>

<!-- <summary> exercises <\summary> -->

a) $3 \cos\theta d\theta$

$= 3 \sin \theta + c$
$$\begin{matrix}\text{c)}\int\frac{4}{5}\sec(x)\tan(x)+x^2\:dx\end{matrix}$$

$$\mathsf{d})\:\int{\frac{\sec^{2}(x)}{3}}+{\frac{1}{\cos^{2}(x)}}dx$$

$$\begin{matrix}\text{f)}\int-\cos\bigl(\theta\bigr)\sin(\theta)\:d\theta\end{matrix}$$

$$\text{g)}\int4\sec^2\begin{pmatrix}x\end{pmatrix}\tan(x)\:dx$$

\<\details\>

------------------------------------------------------------------------

There are other trigonometric functions whose integrals are not so
obvious.

$$\int\tan(x)dx=$$

$$\begin{align*}
\int \tan x \, dx 
&= \int \frac{\sin x}{\cos x} \, dx \\[6pt]
&= \int \frac{1}{\cos x} \sin x \, dx \\[6pt]
\text{Let } t = \cos x \;\;\Rightarrow\;\; &dt = -\sin x \, dx \;\;\Rightarrow\;\; \sin x \, dx = -dt \\[6pt]
&= \int \frac{1}{t} (-dt) \\[6pt]
&= - \int \frac{1}{t} \, dt \\[6pt]
&= -\ln |t| + C \\[6pt]
&= -\ln |\cos x| + C \\[6pt]
&= \ln \left|\frac{1}{\cos x}\right| + C \\[6pt]
&= \ln |\sec x| + C.
\end{align*}$$

OTHER TRIGONOMETRIC INTEGRALS

$$\begin{aligned}\int\tan(x)\:dx&=\\&=\end{aligned}$$

$$\begin{aligned}\int\cot(x)\:dx&=\\&=\end{aligned}$$

$$\int\csc(x)\:dx=\ln\left|\csc(x)-\cot(x)\right|+C$$

$$\int\sec(x)\:dx=\ln\left|\sec(x)+\tan(x)\right|+C$$

Note that $\int\tan(x)dx$ and $\int cot(x)dx$ havetwo forms. Choose the
one that works best for you!

------------------------------------------------------------------------

E2Prove $$\begin{aligned}
\int\cot(x)dx& =\quad\ln\left|\sin\left(x\right)\right|+C \\
&=-\ln\left|\csc(x)\right|+C
\end{aligned}$$

E3 Use the rules to find the following integrals a) $\int4\tan(x)dx$

$$\text{b)}\int\left(-3\cot\left(x\right)-x^3\right)dx$$

a) 3x² sec(x²)dx

a) $9x csc(3x^2) dx$

$$
\begin{align*}
  \text{Let } u = 3x^2 \implies du = 6x dx \\
  \implies \frac{9}{6} \csc \\
\end{align*}
$$

------------------------------------------------------------------------

For integrands we do not recognize as derivatives, some simplification,
identities, or applying the substitution method will help.

### Basic Identities:You must know these

$${\frac{1}{\cos(x)}}\quad\sec(x)={\frac{1}{\cos(x)}}\quad{\frac{\sin(x)}{\cos(x)}}=\quad={\frac{1}{\cos(x)}}$$

$$\csc(x)=\frac{1}{1}$$

Try rewriting with identities:
$$\int\frac{\cos(\theta)}{\sin^2(\theta)}d\theta $$

Try U-Substitution:

$$\begin{align*}
  \int\frac{\cos(\theta)}{\sin^2(\theta)}d\theta \\
  u = \sin\theta \implies du = \cos\theta dx \\
  \implies \int \frac{du}{u^2} \\
  = \int u^{-2} du \\
  = \frac{u^{-1}}{-1} + c \\
  = -\frac{1}{u} + c \\
  = -\frac{1}{\sin\theta} + c \\
  = -\csc\theta + c \\
\end{align*}$$

------------------------------------------------------------------------

E4 Use identities,then find the integral

$$\int\cos^{-2}(x)\sin(x)dx$$

$$\text{c)}\int\frac{\cos(5x)}{\sin(5x)}dx$$

$$
\begin{align*}
  u = 5x \implies du = 5 dx \\
  \frac{1}{5} \int \cot u du \\
  \frac{1}{5} \ln | \sin u | + c\\
\end{align*}
$$

E5 Use u substitution to find the particular solution of
$g(x)=\int\cos^{2}(x)\sin(x)dx$ ,given that $g(\pi)=\frac{4}{3}$

$$
\begin{align*}
  u = \cos x &\implies du = - \sin x dx \\
  \implies G(x) &= - \int u^2 du \\
  G(x) &= - \frac{u^3}{3} + c \\
  G(x) &= - \frac{\cos^3 x}{3} + c \\
  \frac{4}{3} &= - \frac{\cos^3 \pi}{3} + c \\
  c &= \frac{4}{3} + \frac{\cos^3 \pi}{3} \\
  c &= 1 \\
  G(x) &= - \frac{\cos^3 x}{3} + 1 \\
\end{align*}
$$
