---
title: 3. Techniques Of Integration
---

## Videos and Site

Overall review:

{{< video https://www.youtube.com/watch?v=vLdwu6nDWqk >}}

## Integration by Parts

### Videos and sites

{{< video https://www.youtube.com/watch?v=sWSLLO3DS1I >}}

[Integration by Parts: LIPET & LIATE](https://www.kristakingmath.com/integration-by-parts)

### Uni notes

So far we have found antiderivatives when the integral is a derivative

$\int 2xe^x dx$

However, we have a problem when. trying to integrate something like

$\int xe^x dx$

This chapter will look at several advanced techniques for integrals that are not derivatives

For a function $f(x)g(x)$ $$\frac{d}{dx}f(x)g(x)=$$

So, going backwards, we know

$$\int f'(x)g(x)+f(x)g'(x)dx=$$

1

![](./images/f6gpTHnccDETYhS7GwR3skQB2VMgEe3A6.png)

This pattern is not very useful to us. However,we can rearrange it:

$$\int\left[f'\left(x\right)g\left(x\right)+f\left(x\right)g'\left(x\right)\right]dx=f\left(x\right)g\left(x\right)+C\\\int\left[f\left(x\right)g'\left(x\right)\right]dx=f\left(x\right)g\left(x\right)-\int\left[f'\left(x\right)g\left(x\right)\right]dx$$

Our new technique is called integration by parts

Often we use substitution to make the formula easier

Integration by parts is like a“product rule for integration”and has the following formula:

$$\int fg'dx=fg-\int f'gdx\quad\mathrm{or}\quad\int udv=uv-\int vdu$$

We generally choose $f(x)$ or $u$ so that it gets simpler when we take
the derivative of it

<details><summary>Q & A<\summary>

#### E1 Evaluate using Integration by Parts

\begin{align*}
     &\int udv=uv-\int vdu \\
     &\int xe^{x}dx \\
     u = x \to du = dx \\
     dv = e^x dx \to v = \int e^x dx \\
     v = e^x [ C ] \\
     \text{For IBP, we don't need the constant} \\
     = xe^x - \int e^x dx xe^x - e^x + C \\
\end{align*}

### E2 Evaluate using Integrationby Parts

$$\int\frac{x}{-2\left(x-1\right)^3}dx$$

### 3 Evaluate the integral.

$$\int\limits_0^\pi x\sin x\:dx$$

<\details>

### HOW TO CHOOSE u AND dv

The most important step of integration by parts is choosing $f$ or $u$

Remember: We want the function to become easier after taking the
derivative If you struggle to choose. $u$ when expressions get more
complicated, try this:.

LIPET

4-Exponentials 3-Polynomials 5-Trig

1-Logs

2-lnverse Trig

E3 Given the following expressions, state which function is $f$ or $u$
and why

Why?

foru

Special Case E4 Find: $\int\ln(x)dx$

### Table Method: Integration by Parts.

#### Videos and sites

{{< video https://www.youtube.com/watch?v=Yyic5aaXGaw >}}

#### Uni Notes

Some integration by parts questions make us repeat the process more than
once. In these cases it may be useful to organize the parts in a table..

![](./images/fdU7IuuxgtASR0qvzvgrZRZrMIAyDB7lQ.png)

$$\int x^3\cos(x)dx$$

e5 Use the table format of Integration by parts to solve the integral
$$\int e^{2x}(x^3+2x)dx$$

You can still use the tabular method even if neither column hits zero.
You need to incorporate "stops."(Stops are specified criteria that allow
you to continue the process.)First stop:when you hit a zero in one of
the columns.Second:if you can find the integral of the product of a
row.Third: if the product of the row is a multiple of the original
equation.(i.e.positive or negative.)

$$\begin{array}{l}\int x^s\ln(x)dx\\\int e^x\sin(x)dx\end{array}$$

Consider the following:

$$\int x(x-2)^6dx$$

In some cases we can use an extension of u-substitution, algebraic
substitution, to handle cases like this.

$$\int x(x-2)^6dx$$

## GENERAL PROCEDURE FOR ALGEBRAIC SUBSTITUTION

### Videos and Sites

{{< video https://www.youtube.com/watch?v=rsa3bWRoWro >}}

### Uni notes

1.Choose $u$ as the inside funtion 2. Differentiate it to get $du$ 3.
Solve your $u$ equation for $x$ . Use this only for the “extra part" 4.
Substitute everything back into your integral and solve..

Find the integrals using substitution $1\int x{\sqrt{2x-1}}dx$

$$\text{E2}\int\frac{x}{3\left(x+1\right)^{3}}dx\:.$$

$$\text{E3}\int\left(x^2\sqrt{1-x}\right)dx\:.$$

E4 3xx²+4 dx

## Trigonometric Substitution

### Videos and sites

{{< video https://www.youtube.com/watch?v=ocgjfF2AboA >}}

### Uni notes

Consider the following function:

$$\int\frac{1}{\sqrt{1-x^2}}dx$$

Trig substitution lets us get rid of the square root in our expressions.The technique comes from the Pythagorean Theorem:

$$\sin^2\theta+\cos^2\theta=1\quad\tan^2\theta+1=\sec^2\theta $$

We can rewrite them as:

\begin{align*}
  1 - \sin^2 \theta = cos^2 \theta a^2(1 - \sin^2 \theta) = a^2(cos^2 \theta) a^2 - (a \sin \theta)^2 = (a cos \theta)^2 \\
  1 + \tan^2 \theta = \sec^2 \theta a^2(1 + \tan^2 \theta) = a^2(\sec^2 \theta) a^2 + (a \tan \theta)^2 = (a \sec \theta)^2
  \sec^2 \theta - 1 = \tan^2 \theta a^2(\sec^2 \theta - 1) = a^2(\tan^2 \theta) (a \sec \theta)^2 - a^2 = (a \tan \theta)^2 \\
\end{align*}

Let:

If we use the appropriate substitution our radical will disappear:
$$\int\frac{1}{\sqrt{1-x^2}}dx$$

Trigonometric substitution is used when we see a sum or difference of squares in a radical

Let $x=a\sin\theta$

Let x=asec\theta

Let x=atan\theta

Then x²-a²=(atan \theta) Then a + x2 = (asec 0) Then
$a^{2}-x^{2}=(a\cos\theta)^{2}$

These substitutions help us remove the radical and make the integration
easy

### Recognizing the trig substitution

E1 Decide which trigonometric substitution you would use for each
problem and rewrite the integral.
$$\text{b)}\int\frac{2}{\sqrt{4-x^2}}dx$$

a) $\int\frac{dx}{\sqrt{25+x^2}}$

Note:A complete substitution should leave only \theta in the integral, no x.

The radical should disappear, if the substitution is done correctly.

$$\int\frac{1}{x\sqrt{x^{2}-36}}dx$$

\begin{align*}
	\int\frac{1}{x^{2}\sqrt{3-x^{2}}}dx       \\
	\alpha^2 = 3 \implies \alpha = \sqrt{3}   \\
	x  & =\sqrt{3} \sin \theta                \\
	dx & = \sqrt{3} \cos \theta \cdot d\theta \\
\end{align*}

$$\int\frac{1}{x^{2}\sqrt{3-x^{2}}}dx$$

\begin{align*}
	\int\frac{1}{{(\sqrt{3} \sin \theta)}^2 \sqrt{3-{(\sqrt{3} \sin \theta)}^{2}}} \sqrt{3} \cos \theta \cdot d\theta
	            & = \int
	\frac{\cancel{ \sqrt{3} \cos \theta }}{
		3 \sin^2 \theta \cdot \cancel{ \sqrt{3} \cos \theta }
	} d\theta                                                  \\
	= \frac{1}{3} \int \frac{1}{\sin^2 \theta}                 \\
	            & = \frac{1}{3} \int \csc^2 \theta d\theta     \\
	            & = \frac{1}{3} \cot \theta + C                \\
	\sin \theta & = \frac{x}{\sqrt{3}}
	            & = \mathrm{\frac{Opposite\ side}{Hypotenuse}} \\
	\cos \theta & = \frac{\sqrt{3-x^2}}{\sqrt{3}}              \\
	\cot \theta & = \frac{\cos\theta}{\sin\theta}              \\
	            & = \frac{
		\frac{\sqrt{3-x^2}}{\sqrt{3}}
	}{
		\frac{x}{\sqrt{3}}
	}                                                          \\
	            & = \frac{\sqrt{3-x^2}}{x}                     \\
	            & = -\frac{1}{3} \cdot
\end{align*}

### Solving Trig Substitution Integrals

After making a substitution and eliminating the radical:
$$\int\frac{1}{\sqrt{1-x^2}}dx$$

We need to return to the original variable, x

This requires manipulating the original substitution.

Complete the following integrations

E2 $\int\frac{1}{4+x^2}dx$

\begin{align*}
	\int\frac{1}{4+x^2}dx &                       \\
	\alpha^2 + x^2                                \\
	                      & \implies \alpha^2 = 4 \\
	                      & \implies \alpha = 2   \\
	x = 2 \tan \theta                             \\
	                      & \implies \tan \theta  \\
	                      & = \frac{x}{2}         \\
\end{align*}


$$\cdot\int\frac{2}{x\sqrt{x^{2}-36}}dx$$

More complicated integrations are not so easy to return to the original
variable

$$\int\frac{1}{x^2\sqrt{25-x^2}}dx$$

We need to return to the. original variable, x.

This requires manipulating the original substitution.

Remember: When assessing a Definite Integral using substitution, we must
return to the original variable before substituting the bounds

### Evaluate the following integrals using the appropriate trig substitution

E4

$$\int\frac{\sqrt{x^{2}-25}}{x}dx\:x\geq5$$

\begin{align*}
  \int\frac{\sqrt{x^{2}-25}}{x}dx \quad x\geq5 \\
  x^2 - \alpha^2 & \\
                 &\implies \alpha = 5 \\
  x = 5 \sec \theta \\
  dx = 5 \sec\theta \cdot \tan\theta d\theta \\
  \int\frac{\sqrt{5 \sec \theta^{2}-25}}{5 \sec \theta} & 5 \sec\theta \cdot \tan\theta d\theta \\
                                                        & = \int \frac{5 \tan\theta}{5} \cdot \tan\theta d\theta \\
                                                        & = 5 \int \tan^2 \theta d\theta \\
                                                        & = 5 \int [\sec^2 \theta -1] d\theta \\
                                                        & = 5\tan\theta - 5 \theta + C \\
  \cos \theta = \frac{5}{x} \\
  \tan \theta = \frac{\sqrt{x^{2}-25}}{5} \\
                                                        & = 5 \frac{\sqrt{x^{2}-25}}{5} - 5 \sec^{\frac{x}{5}} + C \\
\end{align*}

$${\textrm{s}}\int{\frac{1}{\sqrt{x^{2}+1}}}dx$$

## Partial Fractions

### Videos and sites

{{< video https://www.youtube.com/watch?v=6rXByMcuAyI >}}

### Uni notes

Consider $\int\frac{7-x}{x^2+x-2}dx$

> Structure:
>
> $\frac{Q(x)}{f(x)}$
> $degree(f(x)) > degree(Q(x))$

We can rewrite the integrand using the denominator's factors with the
Partial Fractions method.

### PARTIAL FRACTIONS FOR NON-REPEATED LINEAR FACTORS

If the denominator of an expression can be factored we can use partial
fractions

$$\frac{numerator}{(factor\:1)(factor\:2)}=\frac{A}{(factor\:1)}+\frac{B}{(factor\:2)}$$

Factor the following expression then integrate it using partial
fractions.

$$\int\frac{7-x}{x^2+x-2}dx$$

\begin{align*}
	\int\frac{7-x}{x^2+x-2}dx &                                 \\
	\frac{7-x}{x^2+x-2}       & \implies                        \\
	\frac{7-x}{(x-1)(x+2)}    & = \frac{A}{x-1} + \frac{B}{x+2} \\
	\text{multiply both sides with } (x-1)(x+2)                 \\
	7 - x = A(x+2) + B(x-1)                                     \\
	\text{Long way:}                                            \\
	7 - x = Ax + A2 + Bx - B                                    \\
	\implies 7 -x - Ax - A2 - Bx + B = 0                        \\
	x[-1-A-B]+7+2A-B = 0                                        \\
\end{align*}

Shortcut: choose a value for x that eliminates one of the terms. Then find the remaining term. Then repeat the process for the other term

For A:

\begin{align*}
	x=1 \implies 7-1 = A(1+2) \\
	6 = 3A \implies A =2      \\
\end{align*}

For B:

x = -2


### GENERAL PROCEDURE FOR PARTIAL FRACTIONS

1. Factor the denominator 2. Set up partial fractions 3. Eliminate
    fractions by multiplying though (or using common denominator) 4.
    Solve for your constants (A, B, etc...) 5. Integrate your new,
    simplified expression

Use partial fractions to find the following integrals

E $\int\frac{3x+11}{(x-3)(x+2)}dx\:.$

E2 $\int\frac{x}{x^2+2x-3}dx$

In the previous examples we had a denominator with factors that were
linear terms. In fact they are non- repeating factors

$$\frac{7-x}{x^2+x-2}$$

Has factors

$$\frac{A}{\left(x+2\right)}+\frac{B}{\left(x-1\right)}$$

So ourpartial fraction has the form,

### PARTIAL FRACTIONS FOR REPEATED LINEAR FACTORS

If the denominator of an expression can be factored we can use partial
fractions

$$\frac{numerator}{\left(factor\right)^2}=\frac{A}{\left(factor\right)}+\frac{B}{\left(factor\right)^2}$$

$$\frac{numerator}{\left(factor\right)^2}=\frac{A}{\left(factor\right)}+\frac{B}{\left(factor\right)^2}+\frac{C}{\left(factor\right)^3}+\frac{D}{\left(factor\right)^4}$$

### Repeated Linear Factors

This denominator has a mix of non-repeating and repeating factors

$$\frac{1}{x(x+3)^2}$$

\begin{align*}
	\frac{1}{x(x+3)^2} = \frac{A}{x} + \frac{B}{x+3} + \frac{C}{( x+3 )^2}     \\
	\begin{matrix}
		x = 0           & x = -3           & x = -2                                \\
		\bot = 9A       & \bot = -3C       & \bot = A-2B-2C                        \\
		A = \frac{1}{3} & C = -\frac{1}{3} & \bot = \frac{1}{9} -2{B} +\frac{2}{3} \\
	\end{matrix} \\
	2B = \frac{1}{g}
\end{align*}

{18}-----------

Has factors

So our partial fraction has the form,

Find the following integrals: B $\int\frac{dx}{x\left(x+3\right)^2}$

E4

$$\int\frac{3x^2+24x+37}{\left(x-1\right)\left(x+3\right)^2}dx$$

\begin{align*}
	\int\frac{3x^2+24x+37}{\left(x-1\right)\left(x+3\right)^2}dx                       \\
	\int\frac{3x^2+24x+37}{
		\left(x-1\right)\left(x+3\right)^2
	}dx &                                                                              \\
	    & = \int \left( \frac{A}{x-1} + \frac{B}{x+3} + \frac{C}{( x+3 )^2} \right) dx \\
	    & = A \ln | x-1 | + B \ln | x+3 | + C \ln |x+3| + c                            \\
\end{align*}

### Note:

Fractions where the degree of the numerator is greater than or equal to
the degree of the denominator are called improper or "top-heavy”
fractions.These types of questions would require long division to reduce
the exponent before applying the method of partial fractions Examples of
improper fractions:

$$\frac{9x^2+20x-10}{(x+2)(3x-1)}\frac{2\left(4x^2+1\right)}{(2x+1)(2x-1)}\frac{2x^3+3x^2-2}{(x+2)(x-1)}\frac{x^3-x^2-16x-13}{x^2-3x-10}$$

{19}--------

### NON-REPEATED Quadratic Factors

> When we look at factors that cant be solved with real numbers, we would likely have to use trigonometric substitution

The above concepts also canbe applied where thefactors in the
denominatorare irreducible quadratics.

This works when Which will have $$\int\frac{f(x)}{g(x)}dx$$ we have the
Partial Fractions $$\frac{Ax+B}{g(x)}$$ of theform form:

Find the indefite integral of $\int\frac{4x+4}{x^3+4x}dx$

$$\begin{gathered}
\frac{4x+4}{x^{3}+4x} =\frac{4x+4}{x\Big(x^{2}+4\Big)}=\frac{A}{x}+\frac{Bx+C}{\Big(x^{2}+4\Big)} \\
4x+4 =A\Big(x^{2}+4\Big)+Bx^{2}+Cx 
\end{gathered}$$

$$\begin{aligned}&If\:x=0:\:4=A(4)\:\Rightarrow\:A=\boxed{1}\\&If\:x=1:\quad3=B+C\\&If\:x=-1:\:-5=B-C\end{aligned}$$

$$\begin{bmatrix}1&1\\1&-1\end{bmatrix}\begin{bmatrix}B\\C\end{bmatrix}=\begin{bmatrix}3\\-5\end{bmatrix}\\B=-1,\:C=4$$

Therefore,

$$\begin{aligned}
\int{\frac{4x+4}{x^{3}+4x}}dx& =\int\frac{1}{x}-\frac{x-4}{\left(x^{2}+4\right)}dx  \\
&=\int\frac{1}{x}-\frac{x}{\left(x^{2}+4\right)}+4\frac{1}{4\left(\left(\frac{x}{2}\right)^{2}+1\right)}dx \\
&=\ln\left(x\right)-\frac12\ln\left(x^{2}+4\right)+2\tan^{-1}\left(\frac x2\right)+C
\end{aligned}$$

### Repeated quadratic factors

In the case of repeated quadratic factors in the denominator we apply a
similar technique as case B.Keep in mind that the numerators of the
partial fractions have to have a lower degree than the denominator. This
means that the numerator can possibly be linear expressions.

So for example,

$$\frac{5}{\left(x+1\right)\left(x^2+2x+3\right)^2}=\frac{A}{\left(x+1\right)}+\frac{B_1x+C_1}{\left(x^2+2x+3\right)}+\frac{B_2x+C_2}{\left(x^2+2x+3\right)^2}\:.$$

As before, the task then becomes determining all of the constants

$$\begin{aligned}
& 7{:}\:\mathrm{Find~the~indefinite~integral~of}\:\int\:\frac{2r^{3}}{\left(r^{2}+1\right)^{2}}dr\:.  \\
&\frac{2}{(r^2}& \text{10000} & \frac{r^{*}}{+1)^{2}}=\frac{Ar+B}{\left(r^{2}+1\right)}+\frac{Cr+D}{\left(r^{2}+1\right)^{2}}\quad2r^{3}=Ar^{3}+Br^{2}+\left(A+C\right)r+\left(B+D\right) & \text{-}  \\
&&&2r^{3}& \text{一} && =\left(Ar+B\right)\left(r^{2}+1\right)+Cr+D\quad Equating\:Coefficients && \text{:}  \\
&&&\text{A 3} ^{2r}  2r^{\circ} & =Ar^{3}+Ar+Br^{2}+B+Cr+D && =Ar^{3}+Br^{2}+\left(A+C\right)r+\left(B+D\right) && 4+C=0\quad B+D=0 && A=\boxed{2}\quad B=\boxed{0}  \\
&&C={\boxed{-2}}\quad D={\boxed{0}}
\end{aligned}$$

Therefore,

$$\begin{aligned}
\int\frac{2r^{3}}{\left(r^{2}+1\right)^{2}}dr& =\int\frac{2r}{\left(r^{2}+1\right)}-\frac{2r}{\left(r^{2}+1\right)^{2}}dr  \\
&=\int\frac{1}{\left(r^{2}+1\right)}-\frac{1}{\left(r^{2}+1\right)^{2}}\left(2rdr\right),\:let\:u=r^{2}+1,\:du=2rdr \\
&=\int\frac{1}{u}-\frac{1}{u^{2}}du \\
&=\ln\left(r^{2}+1\right)+\frac{1}{\left(r^{2}+1\right)}+C
\end{aligned}$$

## Improper Integrals

### Definition 1: Improper integrals of Type I

#### Videos and sites

{{< video https://www.youtube.com/watch?v=45YcoKNRa-Y >}}

Organic chemistry tutor (incomplete, watch the other guy's videos):

{{< video https://www.youtube.com/watch?v=ND9cEdfCFr0 >}}

#### Uni notes

Integrals of continuous functions with either one or both of the limits
of integration are infinite are called improper integrals of Type I.

1. If $f(x)$ is continuous on \[a,o), then we define the improper
    integral $\int_a^\infty f(x)dx$ tobe

$$\boxed{\int_a^\infty f(x)\:dx=\lim\limits_{R\to\infty}\int_a^Rf(x)\:dx.}$$

2.If $f(x)$ is continuous on $(-\infty,b]$ , then we define the improper
integral $\int_{-\infty}^bf(x)dx$ tobe

$$\boxed{\int_{-\infty}^af(x)\:dx=\lim\limits_{R\to-\infty}\int_R^af(x)\:dx.}$$

In either case,if the limit exists and equals some value L,we say that
the improperintegral converges to L. If the limit does not exist, we say
that the improper integral diverges

Ex.: Determine whether the following improper integrals converge or
diverge

a) $\int_{1}^{\infty}\frac{1}{\sqrt{x}}dx$

a) $\int_{-\infty}^{-1}\frac{1}{x}dx$

<!-- -->

A) $\int_0^\infty e^{-x}\:dx$

<!-- -->

a) $\int_{-\infty}^0xe^x\:dx$

### L'Hopital's Rule Suppose $\lim_{x\to a}\frac{f\left(x\right)}{g\left(x\right)}=\frac{0}{0}$ or $\lim_{x\to a}\frac{f\left(x\right)}{g\left(x\right)}=\frac{\pm\infty}{\pm\infty}$

Where $a$ can be any real number, infinity or negative infinity. In
these cases we have.
$$\lim_{x\to a}\frac{f\left(x\right)}{g\left(x\right)}=\lim_{x\to a}\frac{f\left(x\right)}{g\left(x\right)}$$

Note: Sometimes you need to apply L'Hopital's Rule more than once.

3.If $f(x)$ is continuous on $(-\infty,\infty)$ , then we define the
improper integral. $\int_{-\infty}^{\infty}f(x)dx$ tobe

![](./images/fQEbYWN5SqVQw4EUDL7Qt1Z4NsfugPRMo.png)

This improper integral $\int_{-\infty}^{\infty}f(x)dx$ converges if and
only if both $\int_{-\infty}^{c}f(x)dx$ and $\int_c^\infty f(x)dx$
converge. If either one diverges, then the original improper integral
$\int_{-\infty}^{\infty}f(x)dx$ also diverges

Ex:Determine whether each of the following improper integrals converge
or diverge.

a) $\int_{-\infty}^{\infty}xe^{-x^2}\:dx$

$<smiles>[24]C(=[2]O)(-[1](-[7](-[1](-[7](-[1](-[7](-[1](-[7](-[1]))))))))))</smiles>$

### Definition 2: Improper integrals of Type II

#### Videos and sites

{{< video https://www.youtube.com/watch?v=w46sjRIkV7Y >}}

#### Uni notes

Integrals of discontinuous functions that become infinite at a point
within the interval of integration. (Infinite discontinuity i.e.
vertical asymptote lies in the interval of integration) are called
improper integrals of Type li.

Examples:

a) 

![](./images/fUImHUs0NhLOTQ7MHpyegrKATgLi8A4Nl.png)

This is not a proper definite integral Since when $x=0$ , the integrand
$\frac{1}{x^2}$ is not definec

![](./images/fQpW7gHxbcfZPVqK49VuqGA15yavIyAMK.png)

a) 

$$\int_0^1\frac{1}{\sqrt{1-x}}\:dx.$$

This is not a proper definite integral as the integrand is undefined at
$x=1$

![](./images/fzEKKNAWDiFRIKwgoprl6xnkILGpyZWQm.png)

1. If $f(x)$ is continuous on (a, b\] and discontinuous at a (i.e
    $|f\left(x\right)|\to\infty$ as $x\to a^{+}$ ), then we. define the
    improper integral $\int_a^bf(x)dx$ to be:

![](./images/fcBT8XgF7xO2FZh3YfZzDL8VrIPGHZzfn.png)

1. If $f(x)$ is continuous on \[a, $b$ ) and discontinuous at $b$ (i.e
    $|f\left(x\right)|\to\infty$ as $x\to b^{-}$ ), then we. define the
    improper integral $\int_a^bf(x)dx$ to be:

$$\boxed{\int_a^bf(x)\:dx=\lim\limits_{R\to b^-}\int_a^Rf(x)\:dx.}$$

In either case 1 or 2, if the limit exists (and equals some value $L$ ),
we say that the impropel integral converges (to $L$ ). If the limit does
not exist,we say that the improper integral diverges

3.If $f(x)$ is continuous on \[a, $b]$ except atsome $c\in(a,b)$ (i.e
$|f\left(x\right)|\to\infty$ as $x\to c$, ,thenwe define the improper
integral $\int_a^bf(x)dx$ to be:

![](./images/fIrIi9htpl2yzTFvmbNlH2rXQvpvulVOn.png)

If both $\int_a^cf(x)dx$ and $\int_c^bf(x)dx$ converge (to $L_{1}$ and
$L_{2}$ , respectively), we say that the improper integral
$\int_a^bf(x)dx$ converges, also (to $L_{1}+L_{2}$

If either of the improper integrals $\int_a^cf(x)dx$ or $\int_c^bf(x)dx$
diverges, then we say that the improper integral $\int_a^bf(x)dx$
diverges, also.

Ex. Determine whether the following improper integrals converge or
diverge.

$$\int_{0}^{1}\frac{1}{\sqrt{1-x}}dx$$

a) $\int_0^1\frac{1}{\sqrt{x}}dx$

<!-- -->

A) $\int_{-1}^{0}\frac{1}{x^{2}}dx$

\begin{align*}
  \lim_{W \to 0^-} \int_{-1}^W \frac{1}{x^2} dx & \\
                                                & = \lim_{W \to 0^-} \frac{}
\end{align*}

a) $$\int_{-1}^2\frac{1}{x^2}dx$$

\begin{align*}
	\int_{-1}^2\frac{1}{x^2}dx & , \quad \text{Discontinuity at 0} \\
	\int
\end{align*}


### e) $\int_{0}^{2}\frac{2x}{x^{2}-4}dx$

![](./images/f00qR61OpXfUvp7OnAFBgWPD1NRSrSCBy.png)

$$)\:\int_{0}^{3}\frac{1}{\left(x-1\right)^{2/3}}dx$$

### Comparison Test

Suppose that $f$ and $g$ are continuous on \[a,) and
$0\leq f\left(x\right)\leq g(x)$ ,for all $x\in[a,\infty)$

(i) If $\int_{a}^{\infty}g(x)\:dx$ converges, thene
    $\int_{a}^{\infty}f(x)\:dx$ converges, also. (i If
    $\int_{a}^{\infty}f(x)\:dx$ diverges, then
    $\int_{a}^{\infty}g\left(x\right)dx$ diverges, also.

The idea of the Comparison Test is to compare a given improper integral
to another. improper integral whose convergence or divergence is already
known (or can be more. easily determined).

The gist:If you're smaller than something that converges, thenyou
converge.

If you're bigger than something that diverges, then you diverge.

Ex.Determine whether the following integrals converge or diverge( Use
the comparison test)

a) $\int_{0}^{\infty}\frac{1}{x+e^{x}}dx\:/(\mathbf{x}\geq0)$

\begin{align*}
  \int_{0}^{\infty}\frac{1}{x+e^{x}}dx\:/(\mathbf{x}\geq0) \\
  \frac{1}{x+e^x} \leq \frac{1}{e^x} \\
  \int_0^\infty \frac{1}{e^x} dx & \\
                                 & = \int_0^\infty e^{-x} dx \\
                                 & = 1 \\
\end{align*}

So due to the comparison test, $\int_0^\infty \frac{1}{e^x} dx$ converges as well

a) $\int_{1}^{\infty}e^{-x^{2}}\:dx$

\begin{align*}
	\int_{1}^{\infty}e^{-x^{2}}\:dx & \\
  \text{Compare } e^{-x} \text{ and } e^{-2x} \\
\end{align*}

a) $\int_{1}^{\infty}\frac{2+\sin\left(x\right)}{\sqrt{x}}dx$

a) $\int_{1}^{\infty}\frac{sin^{2}(x)}{x^{2}}dx$
